Test/SmtTranslation/BitVec.lean
@@ -20,6 +20,7 @@ example (a b : BitVec 10) : a + b = b + a := by
 example (a b c : BitVec 1) : a = b ∨ b = c ∨ c = a := by
   auto
 
+set_option trace.auto.lamReif.prep.printResult true in
 example : (2 : BitVec 7).rotateLeft 3 = (16 : BitVec 7) := by
   auto
 
@@ -27,6 +28,17 @@ example : (2 : BitVec 7).rotateRight 3 = (0x20 : BitVec 7) := by
   auto
 
 example (x : BitVec 15) : x.rotateLeft 3 = x.rotateRight 12 := by
+  auto
+
+example (x : BitVec 20) (y : BitVec 4) :
+  (0#5).rotateLeft x.toNat = 0#5 ∧ (0#5).rotateLeft y.toNat = 0#5 := by
+  auto
+
+example (x : BitVec 20) (y : BitVec 4) :
+  (0#5).rotateRight x.toNat = 0#5 ∧ (0#5).rotateRight y.toNat = 0#5 := by
+  auto
+
+example (x : BitVec 8) : x.rotateLeft (7 - 2 * 2) = x.rotateLeft (1 + 2) := by
   auto
 
 example :
